\section{Derivadas}
\begin{itemize}
	\item $\ds\odv[switch-*,fun=true]{f(x) + g(x)}{x} =\odv[switch-*]{f(x)}{x} +\odv[switch-*]{g(x)}{x}$
	\item $\ds\odv[switch-*]{kf(x)}{x} =k\odv[switch-*]{f(x)}{x}$
	\item $\ds\odv[switch-*]{f(x)g(x)}{x} =f'(x)g(x) + f(x)g'(x)$
	\item $\ds\odv[switch-*,fun=true]{\dfrac{f(x)}{g(x)}}{x} =\dfrac{f'(x)g(x) - f(x)g'(x)}{\pa{g(x)}^{2}}$
	\item $\ds\odv[switch-*]{f(u(x))}{x} =f'(u(x))u'(x)$
	\item $\ds\odv[switch-*]{x}{x} = 1$
	\item $\ds\odv[switch-*]{x^{n}}{x} = nx^{n - 1}$
	\item $\ds\odv[switch-*]{\sqrt[n]{x}}{x} =\dfrac{1}{n\sqrt[n]{x^{n - 1}}}$
	\item $\ds\odv[switch-*]{\sqrt[n]{x^{m}}}{x} =\dfrac{m}{n}\sqrt[n]{x^{m - n}}$
	\item $\ds\odv[switch-*]{\mln{x}}{x} = \dfrac{1}{x}$
	\item $\ds\odv[switch-*]{\mlog{x}[a]}{x} =\dfrac{1}{x\mln{a}}$
	\item $\ds\odv[switch-*]{e^{x}}{x} = e^{x}$
	\item $\ds\odv[switch-*]{a^{x}}{x} = a^{x}\mln{a}$
	\item $\ds\odv[switch-*]{\msin{x}}{x} =\mcos{x}$
	\item $\ds\odv[switch-*]{\mcos{x}}{x} = -\msin{x}$
	\item $\ds\odv[switch-*]{\mtan{x}}{x} =\msec{x}[2]$
	\item $\ds\odv[switch-*]{\mcot{x}}{x} = -\mcsc{x}[2]$
	\item $\ds\odv[switch-*]{\msec{x}}{x} =\msec{x}\mtan{x}$
	\item $\ds\odv[switch-*]{\mcsc{x}}{x} = -\mcsc{x}\mcot{x}$
	\item $\ds\odv[switch-*]{\marcsin{x}}{x} =\dfrac{1}{\sqrt{1 - x^{2}}}$
	\item $\ds\odv[switch-*]{\marccos{x}}{x} = -\dfrac{1}{\sqrt{1 - x^{2}}}$
	\item $\ds\odv[switch-*]{\marctan{x}}{x} =\dfrac{1}{1 + x^{2}}$
	\item $\ds\odv[switch-*]{\marccot{x}}{x} = -\dfrac{1}{1 + x^{2}}$
	\item $\ds\odv[switch-*]{\marcsec{x}}{x} =\dfrac{1}{\abs{x}\sqrt{x^{2} - 1}}$
	\item $\ds\odv[switch-*]{\marccsc{x}}{x} = -\dfrac{1}{\abs{x}\sqrt{x^{2} - 1}}$
\end{itemize}