\section{LÃ­mites}
\begin{itemize}
	\item $\lim\limits_{x\to a}k = k$
	\item $\lim\limits_{x\to a}kf(x) = k\lim\limits_{x\to a}f(x)$
	\item $\lim\limits_{x\to a}\pa{f(x) + g(x)} =\lim\limits_{x\to a}f(x) +\lim\limits_{x\to a}g(x)$
	\item $\lim\limits_{x\to a}f(x)g(x) =\lim\limits_{x\to a}f(x)\lim\limits_{x\to a}g(x)$
	\item $\lim\limits_{x\to a}\dfrac{f(x)}{g(x)} =\dfrac{\lim\limits_{x\to a}f(x)}{\lim\limits_{x\to a}g(x)}$
	\item Sean $F, f:\rmath\to\rmath$ con $F$ continua, entonces:
	\[ \lim\limits_{x\to a}F(f(x)) =F\pa{\lim\limits_{x\to a}f(x)} \]
	\item $\lim\limits_{x\to 0}\dfrac{\msin{kx}}{kx} =\lim\limits_{x\to 0}\dfrac{kx}{\msin{kx}} = 1$
	\item $\lim\limits_{x\to 0}\dfrac{1 -\mcos{x}}{x} = 0$
	\item $\lim\limits_{x\to 0}\dfrac{1 -\mcos{x}}{x^{2}} =\dfrac{1}{2}$
	\item $\lim\limits_{x\to 0}\dfrac{\mtan{kx}}{kx} =\lim\limits_{x\to 0}\dfrac{kx}{\mtan{kx}} = 1$
	\item $\lim\limits_{n\to\infty}\pa{1 +\dfrac{x}{n}}^{n} = e^{x}$
\end{itemize}