\begin{exercise}
	Considere el espacio vectorial $V$ de los polinomios con producto interno definido por $\inprod{f, g} =\mint{f(t)g(t)}{t}[0][1]$ y los polinomios $f(t) = t + 2$, $g(t) = 3t - 2$ y $h(t) = t^{2} - 2t - 3$. Hallar:
	\begin{enumerate}[a)]
		\item $\inprod{f, g}$
		\item $\inprod{f, h}$
		\item $\norm{f}$
	\end{enumerate}
\end{exercise}
\begin{solution}
	\begin{enumerate}[a)]
		\item $\inprod{f, g}$
		\begin{align*}
			\inprod{f, g} &=\mint{f(t)g(t)}{t}[0][1] =\mint{\pa{t + 2}\pa{3t - 2}}{t}[0][1]\\
			&=\mint[1]{3t^{2} + 4t - 4}{t}[0][1]\\
			&=\meval{t^{3} + 2t^{2} - 4t}[0][1]\\
			&= 1^{2} + 2\cdot 1^{2} - 4\cdot 1 = -1
		\end{align*}
		\item $\inprod{f, h}$
		\begin{align*}
			\inprod{f, h} &=\mint{f(t)h(t)}{t}[0][1] =\mint{\pa{t + 2}\pa{t^{2} - 2t - 3}}{t}[0][1]\\
			&=\mint[1]{t^{3} - 7t - 6}{t}[0][1]\\
			&=\meval{\dfrac{1}{4}t^{4} -\dfrac{7}{2}t^{2} - 6t}[0][1]\\
			&=\dfrac{1}{4}\cdot 1^{3} - \dfrac{7}{2}\cdot 1^{2} - 6\cdot 1 = -\dfrac{37}{4}
		\end{align*}
		\item $\norm{f}$
		\begin{align*}
			\norm{f}^{2} &=\mint{f(t)^{2}}{t}[0][1] =\mint{(t + 2)^{2}}{t}[0][1]\\
			&=\mint{u^{2}}{u}[2][3] =\meval{\dfrac{1}{3}u^{3}}[2][3] =\dfrac{1}{3}\pa{3^{3} - 2^{3}} =\dfrac{19}{3}\\
			&\implies\norm{f} =\dfrac{\sqrt{57}}{3}
		\end{align*}
	\end{enumerate}
\end{solution}