\begin{exercise}
	Calcule una base para el subespacio $H$ y para $\mperp{H}$:
	\[  
		H =
		\set{
			\begin{bmatrix}
				x\\
				y\\
				z
			\end{bmatrix}
			\in\rmath[3]: x = y = z
		}
	\]
\end{exercise}
\begin{solution}
	Obtenemos lo siguiente:
	\begin{align*}
		H =\set{
		\begin{bmatrix}
			x\\
			y\\
			z
		\end{bmatrix}
		\in\rmath[3]: x = y = z
		}=\set{
		\begin{bmatrix}
			x\\
			x\\
			x
		\end{bmatrix}
		\in\rmath[3]: x\in\rmath
		}=\set{
		x
		\begin{bmatrix}
			1\\
			1\\
			1
		\end{bmatrix}
		\in\rmath[3]: x\in\rmath
		}=\mgen[1]{\set{
		\begin{bmatrix}
			1\\
			1\\
			1
		\end{bmatrix}
		}}
	\end{align*}
	Por lo que $\set{
		\begin{bmatrix}
			1\\
			1\\
			1
		\end{bmatrix}
	}$ es base de $H$.
	\begin{align*}
		\mperp{H} &=\set{\hat{x}\in\rmath[3]:\forall\hat{y}\in H,\inprod{\hat{x},\hat{y}} = 0}\\
		&=\set{
		\begin{bmatrix}
			a \\ b \\ c
		\end{bmatrix}
		\in\rmath[3]:\forall
		\begin{bmatrix}
			x \\ y \\ z
		\end{bmatrix}
		\in H,
		\begin{bmatrix}
			a \\ b \\ c
		\end{bmatrix}
		\cdot
		\begin{bmatrix}
			x \\ y \\ z
		\end{bmatrix}
		= 0
		}=\set{
		\begin{bmatrix}
			a \\ b \\ c
		\end{bmatrix}
		\in\rmath[3]:\forall x\in\rmath,
		\begin{bmatrix}
			a \\ b \\ c
		\end{bmatrix}
		\cdot
		\begin{bmatrix}
			x \\ x \\ x
		\end{bmatrix}
		= 0
		}\\
		&=\set{
		\begin{bmatrix}
			a \\ b \\ c
		\end{bmatrix}
		\in\rmath[3]:\forall x\in\rmath, ax + bx + cx= 0
		}=\set{
		\begin{bmatrix}
			a \\ b \\ c
		\end{bmatrix}
		\in\rmath[3]:\forall x\in\rmath, (a + b + c)x= 0
		}\\
		&=\set{
		\begin{bmatrix}
			a \\ b \\ c
		\end{bmatrix}
		\in\rmath[3]:a + b + c = 0
		}=\set{
		\begin{bmatrix}
			a \\ b \\ c
		\end{bmatrix}
		\in\rmath[3]:a = -b - c
		}=\set{
		\begin{bmatrix}
			-b - c \\ b \\ c
		\end{bmatrix}
		\in\rmath[3]: b, c\in\rmath
		}\\
		&=\set{
		\begin{bmatrix}
			-b \\ b \\ 0
		\end{bmatrix}
		+
		\begin{bmatrix}
			-c \\ 0 \\ c
		\end{bmatrix}
		\in\rmath[3]: b, c\in\rmath
		}=\set{
		b
		\begin{bmatrix}
			-1 \\ 1 \\ 0
		\end{bmatrix}
		+
		c
		\begin{bmatrix}
			-1 \\ 0 \\ 1
		\end{bmatrix}
		\in\rmath[3]: b, c\in\rmath
		} =\mgen[1]{\set{
		\begin{bmatrix}
			-1 \\ 1 \\ 0
		\end{bmatrix},
		\begin{bmatrix}
			-1 \\ 0 \\ 1
		\end{bmatrix}
		}}
	\end{align*}
	Por lo tanto, $\set{
		\begin{bmatrix}
			-1 \\ 1 \\ 0
		\end{bmatrix},
		\begin{bmatrix}
			-1 \\ 0 \\ 1
		\end{bmatrix}
	}$ es base de $\mperp{H}$.
\end{solution}